# Math 10

*An actually difficult summative test, with new material, in the first week???*

---

## Exponents and Radicals

+ Cube roots are like square roots, but cubes are the products of three equal factors (the root is the value of any of the factors). The operation is represented by a square root symbol but with a small 3 at the top left.
    + You can determine the square or cube root of a perfect square or cube by using prime factorization; make a prime factor tree and divide the prime numbers at the end into either two or three groups, respectively, each with an equal number of each number. Then, multiply all the numbers in a group. (sqrt(729) -> (3, 3, 3) and (3, 3, 3) -> 27)
+ When dealing with negative exponents, continue the pattern of continually dividing the result of the power by the base. (5^2 = 25 -> 25 / 5 = 5 -> 5^1 = 5 -> 5 / 5 = 1 -> 5^0 = 1 -> 1 / 5 = 0.2 -> 5^(-1) = 0.2 -> 0.2 / 5 = 0.04 -> 5^(-2) = 0.04)
    + This can be simplified by dividing 1 by the result of the power but with the exponent made positive. (5^(-1) = 1 / 5^1 = 0.2 -> 5^(-2) = 1 / 5^2 = 0.04)
+ One way of understanding rational non-integer exponents is to consider 25^(1/2) = 5; it can be made into (25^(1/2))^2 = 5^2, which can then be made into 25^1 = 25 using exponent laws. In other words, normal exponent laws apply to rational exponents, and you'll see that on tests.
    + Fractional exponents can be written as radicals. Radicals have the square root symbol, but the number on the inside (the radicand) is the base of the power, and a number to the top left of the radical symbol (the index) is the denominator of the exponent. The radical will then be put into parentheses and raised to the numerator of the exponent.
        + A mixed radical has a radical multiplied by a rational number, while an entire radical is just a radical. A mixed radical can be converted to an entire radical by raising the rational number on the outside by an exponent equal to the radical's index, and then multiplying the radicand by the result. (5 * sqrt(11) = sqrt(5^2) * sqrt(11) = sqrt(5^2 * 11) = sqrt(25 * 11) = sqrt(275))

## Polynomials

+ To multiply polynomials, use the distributive property. You should absolutely be sure to simplify after multiplying when writing a test. ((x - 3)(2x + 1) = x(2x + 1) - 3(2x + 1) = x(2x) + x(1) + -3(2x) + -3(1) = 2x^2 + 1x - 6x - 3 = 2x^2 - 5x - 3)
+ The multiples of a number are the products of some number by a bunch of other numbers. The least common multiple (LCM) of some numbers is the lowest single number that is a possible multiple of all the original numbers (the LCM of 6 and 8 is 24, because 6 * 4 = 24 and 8 * 3 = 24)
+ The factors of a number are the numbers that, when multiplied, yield the original number. Numbers can have many possible factors. The greatest common factor (GCF) of some numbers is the greatest single number that is a possible factor of all the original numbers. (the GCF of 12 and 28 is 4, because 4 * 3 = 12 and 4 * 7 = 28)
    + To get the GCF of a polynomial, you get the GCF from all the terms. The factored form of the polynomial has the GCF multiplying the whole polynomial. (7a^2b - 28ab + 14ab^2 = 7ab(a - 4 + 2b))
        + The GCF of a polynomial can even be another polynomial. (y^2 + 8xy + 2y + 16x = y(y + 8x) + 2(y + 8x) = (y + 8x)(y + 2))
        + When getting the GCF of a polynomial, be sure to factor out any fractions. (1/4a^2 - 2a - 16 = 1/4(a^2 - 8a - 64))
        + When getting the GCF of a polynomial, make sure that the polynomial's parentheses do not begin with negative signs. (-2a + 4b = -2(a - 2b))
    + You can factor out a polynomial by rearranging terms, taking out the GCF, and then grouping. (5x^2 + 18y^2 - 15xy^2 - 6x = 5x^2 - 15xy^2 -6x + 18y^2 = 5x(x - 3y^2) - 6(x - 3y^2) = (x - 3y^2)(5x - 6))
    + Some trinomials can also be factored out by using inspection, or product sum. Say you have a polynomial of the form x^2 + bx + c; you can factor it out by first replacing the bx with two terms whose coefficients have a sum of b and a product of c. Then, factor by grouping. (x^2 + 5x + 6 = x^2 + 3x + 2x + 6 = x(x + 3) + 2(x + 3) = (x + 3)(x + 2), x^2 - x - 12 = x^2 + 3 - 4 - 12 = x(x + 3) - 4(x + 3) = (x + 3)(x - 4))
        + In a similar method, some trinomials of the form ax^2 + bx + c can be factored too, by using decomposition. Replace the bx with two terms whose coefficients have a sum of b and a product of a(c), and then factor by grouping. (3x^2 + 5x - 2 = 3x^2 + 6x - x - 2 = 3x(x + 2) - 1(x + 2) = (x + 2)(3x - 1))
    + A difference of squares, like u^2 - v^2, can be factored into (u + v)(u - v). (s^2 - 9 = (s + 3)(s - 3), 4u^2 - v^2 = (2u + v)(2u - v), p^2/3 - 1 = (p/3 + 1)(p/3 - 1), x^4 - 81 = (x^2 + 9)(x^2 - 9) = (x^2 - 9)(x + 3)(x - 3))
        + Each of these binomial factors in the end result are called conjugate pairs.
